port whnf deciders

pcuic/theories/PCUICInduction.v
@@ -2,6 +2,10 @@
 
 From MetaCoq.Template Require Import utils.
 From MetaCoq.PCUIC Require Import PCUICAst.
+From MetaCoq.PCUIC Require Import PCUICAst PCUICAstUtils PCUICSize.
+Require Import List Program Lia.
+Require Import BinPos.
+Require Import Coq.Arith.Compare_dec Bool.
 Set Asymmetric Patterns.
 
 (** * Deriving a compact induction principle for terms
@@ -58,4 +62,141 @@ Proof.
   fix auxm 1.
   destruct mfix; constructor; [|apply auxm].
   split; apply auxt.
+Defined.
+
+
+Inductive ForallT {A} (P : A -> Type) : list A -> Type :=
+| ForallT_nil : ForallT P []
+| ForallT_cons : forall (x : A) (l : list A), P x -> ForallT P l -> ForallT P (x :: l).
+
+Definition tCaseBrsType {A} (P : A -> Type) (l : list (nat * A)) :=
+  ForallT (fun x => P (snd x)) l.
+
+Definition tFixType {A : Set} (P P' : A -> Type) (m : mfixpoint A) :=
+  ForallT (fun x : def A => P x.(dtype) * P' x.(dbody))%type m.
+
+Lemma size_decompose_app_rec t L :
+  list_size size L + size t = size (decompose_app_rec t L).1 + list_size size (decompose_app_rec t L).2.
+Proof.
+  induction t in L |- *; cbn; try lia.
+  rewrite <- IHt1. cbn. lia.
+Qed.    
+
+Lemma size_decompose_app t :
+  size t = size (decompose_app t).1 + list_size size (decompose_app t).2.
+Proof.
+  unfold decompose_app.
+  eapply (size_decompose_app_rec t []).
+Qed.
+
+Lemma decompose_app_rec_length_mono t L1 L2 :
+  length L1 <= length L2 ->
+  length (decompose_app_rec t L1).2 <= length (decompose_app_rec t L2).2.
+Proof.
+  intros. induction t in L1, L2, H |- *; cbn; try lia.
+  eapply IHt1. cbn. lia.
+Qed.
+
+Lemma decompose_app_rec_length t L :
+  length (decompose_app_rec t L).2 >= length L.
+Proof.
+  induction t in L |- * ; cbn; try lia.
+  unfold ge. etransitivity. eapply IHt1.
+  eapply decompose_app_rec_length_mono. cbn. lia.
+Qed.
+
+Lemma decompose_app_size_tApp1 t1 t2 :
+  size (decompose_app (tApp t1 t2)).1 < size (tApp t1 t2).
+Proof.
+  rewrite size_decompose_app with (t := tApp t1 t2). cbn.
+  pose proof (decompose_app_rec_length t1 [t2]). cbn in H.
+  pose proof (list_size_length size (decompose_app_rec t1 [t2]).2).
+  lia.
+Qed.
+
+Lemma decompose_app_size_tApp2 t1 t2 :
+  Forall (fun t => size t < size (tApp t1 t2)) (decompose_app (tApp t1 t2)).2.
+Proof.
+  todo String.EmptyString.
+Qed.
+
+Definition mkApps_decompose_app_rec t l :
+  mkApps t l = mkApps  (fst (decompose_app_rec t l)) (snd (decompose_app_rec t l)).
+Proof.
+  revert l; induction t; try reflexivity.
+  intro l; cbn in *.
+  transitivity (mkApps t1 ((t2 ::l))). reflexivity.
+  now rewrite IHt1.
+Qed.
+
+Definition mkApps_decompose_app t :
+  t = mkApps  (fst (decompose_app t)) (snd (decompose_app t))
+  := mkApps_decompose_app_rec t [].
+
+Lemma term_forall_mkApps_ind :
+  forall P : term -> Type,
+    (forall n : nat, P (tRel n)) ->
+    (forall i : ident, P (tVar i)) ->
+    (forall (n : nat) (l : list term), All P l -> P (tEvar n l)) ->
+    (forall s, P (tSort s)) ->
+    (forall (n : name) (t : term), P t -> forall t0 : term, P t0 -> P (tProd n t t0)) ->
+    (forall (n : name) (t : term), P t -> forall t0 : term, P t0 -> P (tLambda n t t0)) ->
+    (forall (n : name) (t : term),
+        P t -> forall t0 : term, P t0 -> forall t1 : term, P t1 -> P (tLetIn n t t0 t1)) ->
+    (forall t : term, forall v, ~ isApp t -> P t -> All P v -> P (mkApps t v)) ->
+    (forall (s : kername) (u : list Level.t), P (tConst s u)) ->
+    (forall (i : inductive) (u : list Level.t), P (tInd i u)) ->
+    (forall (i : inductive) (n : nat) (u : list Level.t), P (tConstruct i n u)) ->
+    (forall (p : inductive * nat) (t : term),
+        P t -> forall t0 : term, P t0 -> forall l : list (nat * term),
+            tCaseBrsProp P l -> P (tCase p t t0 l)) ->
+    (forall (s : projection) (t : term), P t -> P (tProj s t)) ->
+    (forall (m : mfixpoint term) (n : nat), tFixProp P P m -> P (tFix m n)) ->
+    (forall (m : mfixpoint term) (n : nat), tFixProp P P m -> P (tCoFix m n)) ->
+    forall t : term, P t.
+Proof.
+  intros until t.
+  assert (Acc (MR lt size) t) by eapply measure_wf, Wf_nat.lt_wf.
+  induction H. rename X14 into auxt. clear H. rename x into t.
+  move auxt at top.
+
+  destruct t; try now repeat (match goal with
+                 H : _ |- _ => apply H; try (hnf; cbn; lia)
+              end).
+
+  - eapply X1. revert l auxt. unfold MR; cbn. fix auxt' 1.
+    destruct l; constructor. apply auxt. hnf; cbn; lia. apply auxt'. intros. apply auxt.
+    hnf in *; cbn in *. lia. 
+
+  - rewrite mkApps_decompose_app.
+    destruct decompose_app eqn:E. cbn.
+    eapply X6.
+    + eapply decompose_app_notApp in E. eauto.
+    + eapply auxt. cbn. hnf. pose proof (decompose_app_size_tApp1 t1 t2). rewrite E in *. hnf in *; cbn in *. lia.
+    + pose proof (decompose_app_size_tApp2 t1 t2). rewrite E in *. cbn in H. clear E.
+      induction l.
+      * econstructor.
+      * econstructor. eapply auxt. hnf; cbn. inv H. eassumption.
+        eapply IHl. inv H. eassumption.
+        
+  - eapply X10; [apply auxt; hnf; cbn; lia.. | ]. rename brs into l.
+    revert l auxt. unfold MR; cbn. fix auxt' 1.
+    destruct l; constructor. apply auxt. hnf; cbn; lia. apply auxt'. intros. apply auxt.
+    hnf in *; cbn in *. lia. 
+  
+  - eapply X12; [apply auxt; hnf; cbn; lia.. | ]. rename mfix into l.
+    revert l auxt. unfold MR; cbn. fix auxt' 1.
+    destruct l; constructor. split.
+    apply auxt. hnf; cbn. unfold def_size. lia.
+    apply auxt. hnf; cbn. unfold def_size. lia.   
+    apply auxt'. intros. apply auxt.
+    hnf in *; cbn in *. unfold mfixpoint_size, def_size in *. lia. 
+
+  - eapply X13; [apply auxt; hnf; cbn; lia.. | ]. rename mfix into l.
+    revert l auxt. unfold MR; cbn. fix auxt' 1.
+    destruct l; constructor. split.
+    apply auxt. hnf; cbn. unfold def_size. lia.
+    apply auxt. hnf; cbn. unfold def_size. lia.   
+    apply auxt'. intros. apply auxt.
+    hnf in *; cbn in *. unfold mfixpoint_size, def_size in *. lia. 
 Defined.
