erasure/theories/SafeTemplateErasure.v
@@ -1,11 +1,34 @@
 (* Distributed under the terms of the MIT license.   *)
 
-From Coq Require Import Bool String Program.
-From MetaCoq.Template Require Import config monad_utils utils uGraph Pretty.
-From MetaCoq.PCUIC Require Import PCUICAst PCUICAstUtils PCUICTyping
-     TemplateToPCUIC.
-From MetaCoq.SafeChecker Require Import PCUICSafeReduce PCUICSafeChecker
-     SafeTemplateChecker.
+From MetaCoq.Erasure Require Import EAst.
+
+Fixpoint opt_cases (t : term) :=
+  match t with
+  | tBox => tBox
+  | tRel n => tRel n
+  | tVar n => tVar n
+  | tEvar n l => tEvar n (List.map opt_cases l)
+  | tLambda na t => tLambda na (opt_cases t)
+  | tLetIn na t1 t2 => tLetIn na (opt_cases t1) (opt_cases t2)
+  | tApp t1 t2 => tApp (opt_cases t1) (opt_cases t2)
+  | tConst k => tConst k
+  | tConstruct i n => tConstruct i n
+  | tCase p tBox ((a, b) :: _) => mkApps b (List.repeat tBox a)
+  | tCase p t brs => tCase p (opt_cases t) (List.map (fun '(n, t) => (n, opt_cases t)) brs)
+  | tProj p t => tProj p (opt_cases t)
+  | tFix mfix id => tFix (List.map (fun d => Build_def term (dname d) (opt_cases (dbody d)) (rarg d)) mfix) id
+  | tCoFix mfix id => tCoFix (List.map (fun d => Build_def term (dname d) (opt_cases (dbody d)) (rarg d)) mfix) id
+  end.
+
+From Coq Require Import Bool String List Program BinPos Compare_dec Arith Lia.
+From MetaCoq.Template Require Import config monad_utils utils BasicAst AstUtils
+     UnivSubst Pretty.
+From MetaCoq.Checker Require Import uGraph Typing.
+From MetaCoq.PCUIC Require Import PCUICAst PCUICAstUtils PCUICInduction
+     PCUICLiftSubst PCUICUnivSubst PCUICTyping PCUICNormal PCUICSR
+     PCUICGeneration PCUICReflect PCUICEquality PCUICInversion PCUICValidity
+     PCUICWeakening PCUICPosition PCUICCumulativity PCUICSafeLemmata PCUICSN TemplateToPCUIC.
+From MetaCoq.SafeChecker Require Import PCUICSafeReduce PCUICSafeConversion PCUICSafeChecker SafeTemplateChecker.
 From MetaCoq.Erasure Require Import ErasureFunction EPretty.
 From MetaCoq.Erasure Require SafeErasureFunction.
 
@@ -18,11 +41,11 @@ Local Open Scope string_scope.
 
 Program Definition erase_template_program_check (p : Ast.program)
   : EnvCheck (EAst.global_context * EAst.term) :=
-  let Σ := (trans_global (Ast.empty_ext p.1)).1 in
+  let Σ := List.rev (trans_global (AstUtils.empty_ext p.1)).1 in
   G <- check_wf_env Σ ;;
-  Σ' <- wrap_error (empty_ext Σ) "erasure of the global context" (erase_global Σ _) ;;
-  t <- wrap_error (empty_ext Σ) ("During erasure of " ++ string_of_term (trans p.2)) (erase (empty_ext Σ) _ nil _ (trans p.2));;
-  ret (Monad:=envcheck_monad) (Σ', t).
+  Σ' <- wrap_error (PCUICAstUtils.empty_ext Σ) "erasure of the global context" (erase_global Σ _) ;;
+  t <- wrap_error (PCUICAstUtils.empty_ext Σ) ("During erasure of " ++ string_of_term (trans p.2)) (erase (empty_ext Σ) _ nil _ (trans p.2));;
+  ret (Monad:=envcheck_monad) (Σ', opt_cases t).
 
 Next Obligation.
   unfold trans_global.
@@ -59,12 +82,13 @@ Program Fixpoint check_wf_env_only_univs (Σ : global_env)
     G <- check_wf_env_only_univs Σ ;;
     check_fresh d.1 Σ ;;
     let udecl := universes_decl_of_decl d.2 in
-    uctx <- check_udecl (string_of_kername d.1) Σ _ G.π1 (proj1 G.π2) udecl ;;
+    uctx <- check_udecl d.1 Σ _ G.π1 (proj1 G.π2) udecl ;;
     let G' := add_uctx uctx.π1 G.π1 in
     assume_wf_decl (Σ, udecl) _ _ G' _ d.1 d.2 ;;
     match udecl with
         | Monomorphic_ctx _ => ret (G'; _)
         | Polymorphic_ctx _ => ret (G.π1; _)
+        | Cumulative_ctx _ => ret (G.π1; _)
         end
     end.
   Next Obligation.
@@ -126,14 +150,27 @@ Program Fixpoint check_wf_env_only_univs (Σ : global_env)
     rewrite eq1; clear eq1.
     assumption.
   Qed.
+  Next Obligation.
+    split; sq. 2: constructor; tas.
+    unfold global_uctx; simpl.
+    assert (eq1: monomorphic_levels_decl g = LevelSet.empty). {
+      destruct g. destruct c, cst_universes; try discriminate; reflexivity.
+      destruct m, ind_universes; try discriminate; reflexivity. }
+    rewrite eq1; clear eq1.
+    assert (eq1: monomorphic_constraints_decl g = ConstraintSet.empty). {
+      destruct g. destruct c, cst_universes; try discriminate; reflexivity.
+      destruct m, ind_universes; try discriminate; reflexivity. }
+    rewrite eq1; clear eq1.
+    assumption.
+  Qed.
 
 Program Definition erase_template_program (p : Ast.program)
   : EnvCheck (EAst.global_context * EAst.term) :=
-  let Σ := (trans_global (Ast.empty_ext p.1)).1 in
+  let Σ := List.rev (trans_global (AstUtils.empty_ext p.1)).1 in
   G <- check_wf_env_only_univs Σ ;;
   Σ' <- (SafeErasureFunction.erase_global Σ _) ;;
   t <- wrap_error (empty_ext Σ) ("During erasure of " ++ string_of_term (trans p.2)) (SafeErasureFunction.erase (empty_ext Σ) _ nil (trans p.2) _);;
-  ret (Monad:=envcheck_monad) (Σ', t).
+  ret (Monad:=envcheck_monad) (Σ', opt_cases t).
 
 Next Obligation.
   unfold trans_global.
@@ -156,8 +193,8 @@ Program Definition erase_and_print_template_program_check {cf : checker_flags} (
   let p := fix_program_universes p in
   match erase_template_program_check p return string + string with
   | CorrectDecl (Σ', t) =>
-    inl ("Environment is well-formed and " ++ Pretty.print_term (Ast.empty_ext p.1) [] true p.2 ++
-         " erases to: " ++ nl ++ print_term Σ' [] true false t)
+    inl ("Environment is well-formed and " ++ Pretty.print_term (AstUtils.empty_ext p.1) [] true p.2 ++
+         " erases to: " ++ nl ++ EPretty.print_term Σ' [] true false t)
   | EnvError Σ' (AlreadyDeclared id) =>
     inr ("Already declared: " ++ id)
   | EnvError Σ' (IllFormedDecl id e) =>
@@ -170,8 +207,8 @@ Program Definition erase_and_print_template_program {cf : checker_flags} (p : As
   let p := fix_program_universes p in
   match erase_template_program p return string + string with
   | CorrectDecl (Σ', t) =>
-    inl ("Environment is well-formed and " ++ Pretty.print_term (Ast.empty_ext p.1) [] true p.2 ++
-         " erases to: " ++ nl ++ print_term Σ' [] true false t)
+    inl ("Environment is well-formed and " ++ Pretty.print_term (AstUtils.empty_ext p.1) [] true p.2 ++
+         " erases to: " ++ nl ++ EPretty.print_term Σ' [] true false t)
   | EnvError Σ' (AlreadyDeclared id) =>
     inr ("Already declared: " ++ id)
   | EnvError Σ' (IllFormedDecl id e) =>
